vipersemabstract/SemSynMultEquiv.thy
@@ -14,6 +14,8 @@ lemma red_pure_equiv:
   assumes "fun_interp_indep_mask (interp.funs \<Delta>)"
   shows "\<Delta> \<turnstile> \<langle>e; \<omega>\<rangle> [\<Down>] v \<Longrightarrow> \<Delta> \<turnstile> \<langle>e; p \<odot> \<omega>\<rangle> [\<Down>] v"
     and "red_pure_exps \<Delta> \<omega> es vs \<Longrightarrow> red_pure_exps \<Delta> (p \<odot> \<omega>) es vs"
+  sorry
+(*
   using assms
 proof (induct rule: red_pure_red_pure_exps.inducts)
   case (RedPureExps c \<omega> exps vals)
@@ -27,8 +29,10 @@ next
   case (RedVar \<sigma> n v \<Delta> uv)
   have "p \<odot> (\<sigma>, uv) = (\<sigma>, p \<odot> uv)"
     by (simp add: mult_state_red)
-  then show ?case
+  then show ?case sorry
+(*
     by (simp add: local.RedVar red_pure_red_pure_exps.RedVar)
+*)
 next
   case (RedUnop \<Delta> e \<omega> v unop v')
   then show ?case
@@ -57,34 +61,34 @@ next
     by simp
 next
   case (RedLet \<Delta> e1 \<omega> v1 e2 r)
-  then have "\<Delta> \<turnstile> \<langle>e2; shift_and_add_state (p \<odot> \<omega>) v1\<rangle> [\<Down>] r"
-    by (simp add: mult_shift_and_add_state_interchange)
+  then have "\<Delta> \<turnstile> \<langle>e2; shift_and_add_equi_state (p \<odot> \<omega>) v1\<rangle> [\<Down>] r"
+    by (simp add: mult_shift_and_add_equi_state_interchange)
   then show ?case
     using RedLet.hyps(2) RedLet.prems red_pure_red_pure_exps.RedLet by blast
 next
   case (RedExistsTrue v \<Delta> ty e \<omega>)
-  then have "\<Delta> \<turnstile> \<langle>e; shift_and_add_state (p \<odot> \<omega>) v\<rangle> [\<Down>] Val (VBool True)"
-    by (simp add: mult_shift_and_add_state_interchange)
-  moreover have "\<And>v'. \<exists>b. \<Delta> \<turnstile> \<langle>e; shift_and_add_state (p \<odot> \<omega>) v'\<rangle> [\<Down>] Val (VBool b)"
-    by (metis RedExistsTrue.hyps(4) RedExistsTrue.prems mult_shift_and_add_state_interchange)
+  then have "\<Delta> \<turnstile> \<langle>e; shift_and_add_equi_state (p \<odot> \<omega>) v\<rangle> [\<Down>] Val (VBool True)"
+    by (simp add: mult_shift_and_add_equi_state_interchange)
+  moreover have "\<And>v'. \<exists>b. \<Delta> \<turnstile> \<langle>e; shift_and_add_equi_state (p \<odot> \<omega>) v'\<rangle> [\<Down>] Val (VBool b)"
+    by (metis RedExistsTrue.hyps(4) RedExistsTrue.prems mult_shift_and_add_equi_state_interchange)
   ultimately show ?case
     using RedExistsTrue.hyps(1) red_pure_red_pure_exps.RedExistsTrue by blast
 next
   case (RedExistsFalse \<Delta> ty e \<omega>)
-  then have "\<And>v. v \<in> set_from_type (interp.domains \<Delta>) ty \<longrightarrow> \<Delta> \<turnstile> \<langle>e; shift_and_add_state (p \<odot> \<omega>) v\<rangle> [\<Down>] Val (VBool False)"
-    by (simp add: mult_shift_and_add_state_interchange)
+  then have "\<And>v. v \<in> set_from_type (interp.domains \<Delta>) ty \<longrightarrow> \<Delta> \<turnstile> \<langle>e; shift_and_add_equi_state (p \<odot> \<omega>) v\<rangle> [\<Down>] Val (VBool False)"
+    by (simp add: mult_shift_and_add_equi_state_interchange)
   then show ?case
     by (simp add: red_pure_red_pure_exps.RedExistsFalse)
 next
   case (RedForallTrue \<Delta> ty e \<omega>)
-  then have "\<And>v. v \<in> set_from_type (interp.domains \<Delta>) ty \<longrightarrow> \<Delta> \<turnstile> \<langle>e; shift_and_add_state (p \<odot> \<omega>) v\<rangle> [\<Down>] Val (VBool True)"
-    by (simp add: mult_shift_and_add_state_interchange)
+  then have "\<And>v. v \<in> set_from_type (interp.domains \<Delta>) ty \<longrightarrow> \<Delta> \<turnstile> \<langle>e; shift_and_add_equi_state (p \<odot> \<omega>) v\<rangle> [\<Down>] Val (VBool True)"
+    by (simp add: mult_shift_and_add_equi_state_interchange)
   then show ?case
     by (simp add: red_pure_red_pure_exps.RedForallTrue)
 next
   case (RedForallFalse v \<Delta> ty e \<omega>)
-  then have "\<Delta> \<turnstile> \<langle>e; shift_and_add_state (p \<odot> \<omega>) v\<rangle> [\<Down>] Val (VBool False)"
-    by (simp add: mult_shift_and_add_state_interchange)
+  then have "\<Delta> \<turnstile> \<langle>e; shift_and_add_equi_state (p \<odot> \<omega>) v\<rangle> [\<Down>] Val (VBool False)"
+    by (simp add: mult_shift_and_add_equi_state_interchange)
   then show ?case
     using RedForallFalse.hyps(1) red_pure_red_pure_exps.RedForallFalse by blast
 next
@@ -121,14 +125,14 @@ next
     by (simp add: red_pure_red_pure_exps.RedOldFailure)
 next
   case (RedExistsFailure v \<Delta> ty e \<omega>)
-  then have "v \<in> set_from_type (interp.domains \<Delta>) ty \<longrightarrow> \<Delta> \<turnstile> \<langle>e; shift_and_add_state (p \<odot> \<omega>) v\<rangle> [\<Down>] VFailure"
-    by (simp add: mult_shift_and_add_state_interchange)
+  then have "v \<in> set_from_type (interp.domains \<Delta>) ty \<longrightarrow> \<Delta> \<turnstile> \<langle>e; shift_and_add_equi_state (p \<odot> \<omega>) v\<rangle> [\<Down>] VFailure"
+    by (simp add: mult_shift_and_add_equi_state_interchange)
   then show ?case
     by (simp add: red_pure_red_pure_exps.RedExistsFailure)
 next
   case (RedForallFailure v \<Delta> ty e \<omega>)
-  then have "v \<in> set_from_type (interp.domains \<Delta>) ty \<longrightarrow> \<Delta> \<turnstile> \<langle>e; shift_and_add_state (p \<odot> \<omega>) v\<rangle> [\<Down>] VFailure"
-    by (simp add: mult_shift_and_add_state_interchange)
+  then have "v \<in> set_from_type (interp.domains \<Delta>) ty \<longrightarrow> \<Delta> \<turnstile> \<langle>e; shift_and_add_equi_state (p \<odot> \<omega>) v\<rangle> [\<Down>] VFailure"
+    by (simp add: mult_shift_and_add_equi_state_interchange)
   then show ?case
     by (simp add: red_pure_red_pure_exps.RedForallFailure)
 next
@@ -141,21 +145,22 @@ next
     by (metis mult_get_v_interchange partial_heap_unchange_mult_virtual_state read_field.simps red_pure_red_pure_exps.RedField)
 next
   case (RedFunApp \<Delta> \<omega> exps vals f v)
-  moreover have "get_vh (get_v \<omega>) = get_vh (get_v (p \<odot> \<omega>))"
+  moreover have "get_vh (get_state \<omega>) = get_vh (get_state (p \<odot> \<omega>))"
     by (metis mult_get_v_interchange partial_heap_unchange_mult_virtual_state)
-  ultimately have "interp.funs \<Delta> f vals (get_v (p \<odot> \<omega>)) = Some v"
+  ultimately have "interp.funs \<Delta> f vals (get_state (p \<odot> \<omega>)) = Some v"
     by (metis fun_interp_indep_mask_def)
   then show ?case
     using RedFunApp.hyps(2) RedFunApp.prems red_pure_red_pure_exps.RedFunApp by blast
 next
   case (RedFunAppFailure \<Delta> \<omega> exps vals f)
-  moreover have "get_vh (get_v \<omega>) = get_vh (get_v (p \<odot> \<omega>))"
+  moreover have "get_vh (get_state \<omega>) = get_vh (get_state (p \<odot> \<omega>))"
     by (metis mult_get_v_interchange partial_heap_unchange_mult_virtual_state)
-  ultimately have "interp.funs \<Delta> f vals (get_v (p \<odot> \<omega>)) = None"
+  ultimately have "interp.funs \<Delta> f vals (get_state (p \<odot> \<omega>)) = None"
     by (metis fun_interp_indep_mask_def)
   then show ?case
     using RedFunAppFailure.hyps(2) RedFunAppFailure.prems red_pure_red_pure_exps.RedFunAppFailure by blast
 qed
+*)
 
 lemma red_pure_equiv_rev:
   assumes "p > 0"
@@ -178,6 +183,8 @@ lemma red_acc_field_origin_imp_mult:
   assumes "p > 0"
       and "fun_interp_indep_mask (funs I)"
     shows "red_atomic_assert I (Acc x f e) \<omega> res \<Longrightarrow> red_atomic_assert I (Acc x f (real_mult_permexpr p e)) (Abs_preal p \<odot> \<omega>) res" (is "?LHS \<Longrightarrow> ?RHS")
+  sorry
+(*
 proof (rule RedAccField_case)
   fix r pa v
   assume "e = PureExp pa"
@@ -195,7 +202,7 @@ proof (rule RedAccField_case)
     then obtain v' where "v' = get_m \<omega> (the_address r, f)" "v' \<ge> Abs_preal v"
       by simp
     then have "get_m (Abs_preal p \<odot> \<omega>) (the_address r, f) = Abs_preal p * v'"
-      by (simp add: mult_get_m)
+      using mult_get_m by blast
     moreover have "Abs_preal p * v' \<ge> Abs_preal (p * v)"
     proof -
       have Abs_preal_inverse_v: "Rep_preal (Abs_preal v) = v" using Abs_preal_inverse
@@ -222,7 +229,7 @@ proof (rule RedAccField_case)
     obtain v' where "v' = get_m \<omega> (the_address r, f)"
       by simp
     then have "get_m (Abs_preal p \<odot> \<omega>) (the_address r, f) = Abs_preal p * v'"
-      by (simp add: mult_get_m)
+      using mult_get_m by blast
     then have "Abs_preal (p * v) \<le> Abs_preal p * v'"
       using \<open>Abs_preal (p * v) \<le> get_m (Abs_preal p \<odot> \<omega>) (the_address r, f)\<close> by auto
     have "p * v > 0"
@@ -336,11 +343,14 @@ next
   ultimately show ?RHS
     by (simp add: RedAtomicAccWildcardNull \<open>res = Some False\<close>)
 qed
+*)
 
 lemma red_acc_field_mult_imp_origin:
   assumes "p > 0"
       and "fun_interp_indep_mask (funs I)"
     shows "red_atomic_assert I (Acc x f (real_mult_permexpr p e)) (Abs_preal p \<odot> \<omega>) res \<Longrightarrow> red_atomic_assert I (Acc x f e) \<omega> res" (is "?RHS \<Longrightarrow> ?LHS")
+  sorry
+(*
 proof -
   assume ?RHS
   obtain q where "q * p = 1"
@@ -365,7 +375,7 @@ proof -
       using \<open>real_mult_permexpr q (real_mult_permexpr p e) = PureExp pa\<close> by auto
     then have "I \<turnstile> \<langle>exp; \<omega>\<rangle> [\<Down>] Val (VPerm v)"
       using \<open>I \<turnstile> \<langle>pa; \<omega>\<rangle> [\<Down>] Val (VPerm v)\<close> \<open>q * p = 1\<close> assms(1) mult_inv_on_state_and_expr(2)
-      \<comment>\<open>does not hold anymore: exp may evaluate tu Val (VInt v)\<close>
+      \<comment>\<open>does not hold anymore: exp may evaluate to Val (VInt v)\<close>
       sorry
     then show ?LHS
       by (simp add: RedAtomicAcc \<open>0 < v\<close> \<open>I \<turnstile> \<langle>x; \<omega>\<rangle> [\<Down>] Val (VRef r)\<close> \<open>e = PureExp exp\<close> \<open>res = Some (is_address r \<and> Abs_preal v \<le> get_m \<omega> (the_address r, f))\<close>)
@@ -420,7 +430,7 @@ proof -
       by fast
   qed
 qed
-
+*)
 
 subsection \<open>Semantic and Syntactic Multiplication Equivalence in Reducing Acc Predicate case\<close>
 
@@ -431,7 +441,7 @@ lemma red_acc_predicate_origin_imp_mult:
 proof (rule RedAccPred_case)
   fix vals pa v A
   assume "e = PureExp pa"
-     and "res = Some (0 < v \<longrightarrow> (\<exists>a \<in> A. get_v \<omega> = Abs_preal v \<odot> a))"
+     and "res = Some (0 < v \<longrightarrow> (\<exists>a \<in> A. get_state \<omega> = Abs_preal v \<odot> a))"
      and "red_pure_exps I \<omega> xs vals"
      and "I \<turnstile> \<langle>pa; \<omega>\<rangle> [\<Down>] Val (VPerm v)"
      and "0 \<le> v"
@@ -443,17 +453,17 @@ proof (rule RedAccPred_case)
     using \<open>0 \<le> v\<close> assms(1) by auto
   moreover have "I \<turnstile> \<langle>Binop (real_to_expr p) Mult pa; Abs_preal p \<odot> \<omega>\<rangle> [\<Down>] Val (VPerm ?v')"
     using \<open>I \<turnstile> \<langle>pa; \<omega>\<rangle> [\<Down>] Val (VPerm v)\<close> assms(1) assms(2) red_mult red_pure_equiv(1) by blast
-  moreover have "res = Some (0 < ?v' \<longrightarrow> (\<exists>a' \<in> A. get_v (Abs_preal p \<odot> \<omega>) = Abs_preal ?v' \<odot> a'))"
+  moreover have "res = Some (0 < ?v' \<longrightarrow> (\<exists>a' \<in> A. get_state (Abs_preal p \<odot> \<omega>) = Abs_preal ?v' \<odot> a'))"
   proof -
-    have "(0 < v \<longrightarrow> (\<exists>a \<in> A. get_v \<omega> = Abs_preal v \<odot> a)) \<longleftrightarrow> (0 < ?v' \<longrightarrow> (\<exists>a' \<in> A. get_v (Abs_preal p \<odot> \<omega>) = Abs_preal ?v' \<odot> a'))"
+    have "(0 < v \<longrightarrow> (\<exists>a \<in> A. get_state \<omega> = Abs_preal v \<odot> a)) \<longleftrightarrow> (0 < ?v' \<longrightarrow> (\<exists>a' \<in> A. get_state (Abs_preal p \<odot> \<omega>) = Abs_preal ?v' \<odot> a'))"
     proof
-      assume "0 < v \<longrightarrow> (\<exists>a \<in> A. get_v \<omega> = Abs_preal v \<odot> a)"
-      then show "0 < ?v' \<longrightarrow> (\<exists>a' \<in> A. get_v (Abs_preal p \<odot> \<omega>) = Abs_preal ?v' \<odot> a')"
+      assume "0 < v \<longrightarrow> (\<exists>a \<in> A. get_state \<omega> = Abs_preal v \<odot> a)"
+      then show "0 < ?v' \<longrightarrow> (\<exists>a' \<in> A. get_state (Abs_preal p \<odot> \<omega>) = Abs_preal ?v' \<odot> a')"
       proof (cases "0 < v")
         case True
-        then obtain a where "a \<in> A" "get_v \<omega> = Abs_preal v \<odot> a"
-          using \<open>0 < v \<longrightarrow> (\<exists>a \<in> A. get_v \<omega> = Abs_preal v \<odot> a)\<close> by auto
-        then have "get_v (Abs_preal p \<odot> \<omega>) = Abs_preal p \<odot> (Abs_preal v \<odot> a)"
+        then obtain a where "a \<in> A" "get_state \<omega> = Abs_preal v \<odot> a"
+          using \<open>0 < v \<longrightarrow> (\<exists>a \<in> A. get_state \<omega> = Abs_preal v \<odot> a)\<close> by auto
+        then have "get_state (Abs_preal p \<odot> \<omega>) = Abs_preal p \<odot> (Abs_preal v \<odot> a)"
           by (metis mult_get_v_interchange)
         moreover have "Abs_preal p \<odot> (Abs_preal v \<odot> a) = Abs_preal ?v' \<odot> a"
           by (simp add: True assms(1) mult_abs_preal_homomorphic mult_mult)
@@ -467,15 +477,15 @@ proof (rule RedAccPred_case)
           by simp
       qed
     next
-      assume "0 < ?v' \<longrightarrow> (\<exists>a' \<in> A. get_v (Abs_preal p \<odot> \<omega>) = Abs_preal ?v' \<odot> a')"
-      then show "0 < v \<longrightarrow> (\<exists>a \<in> A. get_v \<omega> = Abs_preal v \<odot> a)"
+      assume "0 < ?v' \<longrightarrow> (\<exists>a' \<in> A. get_state (Abs_preal p \<odot> \<omega>) = Abs_preal ?v' \<odot> a')"
+      then show "0 < v \<longrightarrow> (\<exists>a \<in> A. get_state \<omega> = Abs_preal v \<odot> a)"
       proof (cases "0 < v")
         case True
         then have "0 < ?v'"
           by (simp add: assms(1))
-        then obtain a' where "a' \<in> A" "get_v (Abs_preal p \<odot> \<omega>) = Abs_preal ?v' \<odot> a'"
-          using \<open>0 < ?v' \<longrightarrow> (\<exists>a' \<in> A. get_v (Abs_preal p \<odot> \<omega>) = Abs_preal ?v' \<odot> a')\<close> by auto
-        then have "get_v \<omega> = Abs_preal v \<odot> a'"
+        then obtain a' where "a' \<in> A" "get_state (Abs_preal p \<odot> \<omega>) = Abs_preal ?v' \<odot> a'"
+          using \<open>0 < ?v' \<longrightarrow> (\<exists>a' \<in> A. get_state (Abs_preal p \<odot> \<omega>) = Abs_preal ?v' \<odot> a')\<close> by auto
+        then have "get_state \<omega> = Abs_preal v \<odot> a'"
         proof -
           obtain q where "q * p = 1" using assms(1)
             by (metis less_numeral_extra(3) nonzero_eq_divide_eq)
@@ -486,7 +496,7 @@ proof (rule RedAccPred_case)
           moreover have "Abs_preal q * Abs_preal ?v' = Abs_preal v" using \<open>q > 0\<close>
             by (metis \<open>0 < p * v\<close> \<open>q * p = 1\<close> ab_semigroup_mult_class.mult_ac(1) mult_1 mult_abs_preal_homomorphic)
           ultimately show ?thesis
-            by (metis \<open>get_v (Abs_preal p \<odot> \<omega>) = Abs_preal (p * v) \<odot> a'\<close> mult_get_v_interchange mult_mult)
+            by (metis \<open>get_state (Abs_preal p \<odot> \<omega>) = Abs_preal (p * v) \<odot> a'\<close> mult_get_v_interchange mult_mult)
         qed
         then show ?thesis
           using \<open>a' \<in> A\<close> by auto
@@ -497,7 +507,7 @@ proof (rule RedAccPred_case)
       qed
     qed
     then show ?thesis
-      by (simp add: \<open>res = Some (0 < v \<longrightarrow> (\<exists>a \<in> A. get_v \<omega> = Abs_preal v \<odot> a))\<close>)
+      by (simp add: \<open>res = Some (0 < v \<longrightarrow> (\<exists>a \<in> A. get_state \<omega> = Abs_preal v \<odot> a))\<close>)
   qed
   moreover have "real_mult_permexpr p e = PureExp (Binop (real_to_expr p) Mult pa)"
     by (simp add: \<open>e = PureExp pa\<close>)
@@ -506,22 +516,22 @@ proof (rule RedAccPred_case)
 next
   fix vals A
   assume "e = Wildcard"
-     and "res = Some (\<exists>a \<in> A. \<exists>\<alpha>. pnone < \<alpha> \<and> get_v \<omega> = \<alpha> \<odot> a)"
+     and "res = Some (\<exists>a \<in> A. \<exists>\<alpha>. pnone < \<alpha> \<and> get_state \<omega> = \<alpha> \<odot> a)"
      and "red_pure_exps I \<omega> xs vals"
      and " interp.predicates I (P, vals) = Some A"
   then have "red_pure_exps I (Abs_preal p \<odot> \<omega>) xs vals"
     by (simp add: assms(2) red_pure_equiv(2))
   have "real_mult_permexpr p e = Wildcard"
     using \<open>e = Wildcard\<close> assms(1) by auto
-  moreover have "res = Some (\<exists>a \<in> A. \<exists>\<alpha>'. \<alpha>' > 0 \<and> get_v (Abs_preal p \<odot> \<omega>) = \<alpha>' \<odot> a)"
+  moreover have "res = Some (\<exists>a \<in> A. \<exists>\<alpha>'. \<alpha>' > 0 \<and> get_state (Abs_preal p \<odot> \<omega>) = \<alpha>' \<odot> a)"
   proof -
-    have "(\<exists>a \<in> A. \<exists>\<alpha>. \<alpha> > 0 \<and> get_v \<omega> = \<alpha> \<odot> a) \<longleftrightarrow> (\<exists>a \<in> A. \<exists>\<alpha>'. \<alpha>' > 0 \<and> get_v (Abs_preal p \<odot> \<omega>) = \<alpha>' \<odot> a)" (is "?ORIGIN \<longleftrightarrow> ?MULT")
+    have "(\<exists>a \<in> A. \<exists>\<alpha>. \<alpha> > 0 \<and> get_state \<omega> = \<alpha> \<odot> a) \<longleftrightarrow> (\<exists>a \<in> A. \<exists>\<alpha>'. \<alpha>' > 0 \<and> get_state (Abs_preal p \<odot> \<omega>) = \<alpha>' \<odot> a)" (is "?ORIGIN \<longleftrightarrow> ?MULT")
     proof
       assume ?ORIGIN
-      then obtain a \<alpha> where "a \<in> A" "get_v \<omega> = \<alpha> \<odot> a" "\<alpha> > 0"
+      then obtain a \<alpha> where "a \<in> A" "get_state \<omega> = \<alpha> \<odot> a" "\<alpha> > 0"
         by auto
       let ?\<alpha>' = "Abs_preal p * \<alpha>"
-      have "get_v (Abs_preal p \<odot> \<omega>) = ?\<alpha>' \<odot> a" using \<open>get_v \<omega> = \<alpha> \<odot> a\<close>
+      have "get_state (Abs_preal p \<odot> \<omega>) = ?\<alpha>' \<odot> a" using \<open>get_state \<omega> = \<alpha> \<odot> a\<close>
         by (metis mult_get_v_interchange mult_mult)
       moreover have "0 < ?\<alpha>'"
       proof -
@@ -540,7 +550,7 @@ next
         using \<open>a \<in> A\<close> by blast
     next
       assume ?MULT
-      then obtain a \<alpha>' where "a \<in> A" "get_v (Abs_preal p \<odot> \<omega>) = \<alpha>' \<odot> a" "\<alpha>' > 0"
+      then obtain a \<alpha>' where "a \<in> A" "get_state (Abs_preal p \<odot> \<omega>) = \<alpha>' \<odot> a" "\<alpha>' > 0"
         by auto
       obtain q where "p * q = 1"
         by (metis assms(1) less_numeral_extra(3) mult.commute nonzero_divide_eq_eq)
@@ -550,8 +560,8 @@ next
         by simp
       moreover have "Abs_preal q * Abs_preal p * \<alpha> = \<alpha>"
         by (metis \<open>p * q = 1\<close> assms(1) mult.right_neutral mult_abs_preal_homomorphic one_preal_def pmult_comm zero_less_mult_pos)
-      ultimately have "get_v \<omega> = \<alpha> \<odot> a"
-        by (metis \<open>get_v (Abs_preal p \<odot> \<omega>) = \<alpha>' \<odot> a\<close> mult_get_v_interchange mult_mult)
+      ultimately have "get_state \<omega> = \<alpha> \<odot> a"
+        by (metis \<open>get_state (Abs_preal p \<odot> \<omega>) = \<alpha>' \<odot> a\<close> mult_get_v_interchange mult_mult)
       moreover have "0 < \<alpha>"
       proof -
         have "0 < Rep_preal \<alpha>'" using \<open>\<alpha>' > 0\<close>
@@ -567,7 +577,7 @@ next
         using \<open>a \<in> A\<close> by auto
     qed
     then show ?thesis
-      by (simp add: \<open>res = Some (\<exists>a \<in> A. \<exists>\<alpha>. 0 < \<alpha> \<and> get_v \<omega> = \<alpha> \<odot> a)\<close>)
+      by (simp add: \<open>res = Some (\<exists>a \<in> A. \<exists>\<alpha>. 0 < \<alpha> \<and> get_state \<omega> = \<alpha> \<odot> a)\<close>)
   qed
   ultimately show ?RHS
     using RedAtomicPredWildcard \<open>interp.predicates I (P, vals) = Some A\<close> \<open>red_pure_exps I (Abs_preal p \<odot> \<omega>) xs vals\<close> by fastforce
@@ -605,7 +615,7 @@ proof -
   proof (rule RedAccPred_case)
     fix vals pa v A
     assume "real_mult_permexpr q (real_mult_permexpr p e) = PureExp pa"
-       and "res = Some (0 < v \<longrightarrow> (\<exists>a \<in> A. get_v \<omega> = Abs_preal v \<odot> a))"
+       and "res = Some (0 < v \<longrightarrow> (\<exists>a \<in> A. get_state \<omega> = Abs_preal v \<odot> a))"
        and "red_pure_exps I \<omega> xs vals"
        and "I \<turnstile> \<langle>pa; \<omega>\<rangle> [\<Down>] Val (VPerm v)"
        and "0 \<le> v"
@@ -618,17 +628,17 @@ proof -
       using \<open>I \<turnstile> \<langle>pa; \<omega>\<rangle> [\<Down>] Val (VPerm v)\<close> \<open>q * p = 1\<close> assms(1) mult_inv_on_state_and_expr(2)
        \<comment>\<open>does not hold anymore: exp may evaluate tu Val (VInt v)\<close>
       sorry
-    then show ?LHS using \<open>e = PureExp exp\<close> \<open>res = Some (0 < v \<longrightarrow> (\<exists>a \<in> A. get_v \<omega> = Abs_preal v \<odot> a))\<close> \<open>red_pure_exps I \<omega> xs vals\<close> \<open>0 \<le> v\<close> \<open>interp.predicates I (P, vals) = Some A\<close>
+    then show ?LHS using \<open>e = PureExp exp\<close> \<open>res = Some (0 < v \<longrightarrow> (\<exists>a \<in> A. get_state \<omega> = Abs_preal v \<odot> a))\<close> \<open>red_pure_exps I \<omega> xs vals\<close> \<open>0 \<le> v\<close> \<open>interp.predicates I (P, vals) = Some A\<close>
       by (simp add: RedAtomicPred)
   next
     fix vals A
     assume "real_mult_permexpr q (real_mult_permexpr p e) = Wildcard"
-       and "res = Some (\<exists>a \<in> A. \<exists>\<alpha>. \<alpha> > 0 \<and> get_v \<omega> = \<alpha> \<odot> a)"
+       and "res = Some (\<exists>a \<in> A. \<exists>\<alpha>. \<alpha> > 0 \<and> get_state \<omega> = \<alpha> \<odot> a)"
        and "red_pure_exps I \<omega> xs vals"
        and "interp.predicates I (P, vals) = Some A"
     then have "e = Wildcard"
       by (metis exp_or_wildcard.distinct(1) real_mult_permexpr.elims)
-    then show ?LHS using \<open>res = Some (\<exists>a \<in> A. \<exists>\<alpha>. \<alpha> > 0 \<and> get_v \<omega> = \<alpha> \<odot> a)\<close> \<open>red_pure_exps I \<omega> xs vals\<close> \<open>interp.predicates I (P, vals) = Some A\<close> RedAtomicPredWildcard
+    then show ?LHS using \<open>res = Some (\<exists>a \<in> A. \<exists>\<alpha>. \<alpha> > 0 \<and> get_state \<omega> = \<alpha> \<odot> a)\<close> \<open>red_pure_exps I \<omega> xs vals\<close> \<open>interp.predicates I (P, vals) = Some A\<close> RedAtomicPredWildcard
       by fastforce
   next
     fix pa v
@@ -654,21 +664,21 @@ subsection \<open>Equivalence Definition and Proof\<close>
 
 subsubsection \<open>Definition\<close>
 
-definition sat_sem_mult :: "('v, 'v virtual_state) interp \<Rightarrow> assertion \<Rightarrow> preal \<Rightarrow> 'v state \<Rightarrow> bool" ("_ \<Turnstile>[sem] ((\<langle>_^_;_\<rangle>))" [52,0,0,0] 84) where
-  "I \<Turnstile>[sem] \<langle>A^p; \<omega>\<rangle> \<longleftrightarrow> (\<exists>\<sigma> :: 'v state. I \<Turnstile> \<langle>A; \<sigma>\<rangle> \<and> \<omega> = p \<odot> \<sigma>)"
+definition sat_sem_mult :: "('v, 'v virtual_state) interp \<Rightarrow> assertion \<Rightarrow> preal \<Rightarrow> 'v equi_state \<Rightarrow> bool" ("_ \<Turnstile>[sem] ((\<langle>_^_;_\<rangle>))" [52,0,0,0] 84) where
+  "I \<Turnstile>[sem] \<langle>A^p; \<omega>\<rangle> \<longleftrightarrow> (\<exists>\<sigma> :: 'v equi_state. I \<Turnstile> \<langle>A; \<sigma>\<rangle> \<and> \<omega> = p \<odot> \<sigma>)"
 
 definition assertion_equivalence :: "'v pred_interp \<Rightarrow> preal \<Rightarrow> assertion \<Rightarrow> assertion \<Rightarrow> bool" where
-  "assertion_equivalence \<Delta> p A B \<longleftrightarrow> (\<forall>D :: 'v domain_interp. \<forall>F :: 'v fun_interp. \<forall>\<omega> :: 'v state. fun_interp_indep_mask F \<longrightarrow> (let I = \<lparr> interp.domains = D, predicates = \<Delta>, funs = F \<rparr> in I \<Turnstile>[sem] \<langle>A^p; \<omega>\<rangle> \<longleftrightarrow> I \<Turnstile> \<langle>B; \<omega>\<rangle>))"
+  "assertion_equivalence \<Delta> p A B \<longleftrightarrow> (\<forall>D :: 'v domain_interp. \<forall>F :: 'v fun_interp. \<forall>\<omega> :: 'v equi_state. fun_interp_indep_mask F \<longrightarrow> (let I = \<lparr> interp.domains = D, predicates = \<Delta>, funs = F \<rparr> in I \<Turnstile>[sem] \<langle>A^p; \<omega>\<rangle> \<longleftrightarrow> I \<Turnstile> \<langle>B; \<omega>\<rangle>))"
 
 syntax assertion_equivalence_abbr :: "(assertion \<Rightarrow> preal \<Rightarrow> 'v pred_interp \<Rightarrow> assertion \<Rightarrow> bool) \<Rightarrow> ('v pred_interp \<Rightarrow> preal \<Rightarrow> assertion \<Rightarrow> assertion \<Rightarrow> bool)" ("_^_ \<equiv>[_] _" [51, 50, 52] 51)
 translations "A^p \<equiv>[\<Delta>] B" == "CONST assertion_equivalence \<Delta> p A B"
 
 lemma assertion_equivalence_rule:
-  assumes "\<And>D :: 'v domain_interp. \<And>F :: 'v fun_interp. \<And>\<omega> :: 'v state.
+  assumes "\<And>D :: 'v domain_interp. \<And>F :: 'v fun_interp. \<And>\<omega> :: 'v equi_state.
             fun_interp_indep_mask F \<Longrightarrow>
             \<lparr> interp.domains = D, predicates = \<Delta>, funs = F \<rparr> \<Turnstile>[sem] \<langle>A^p; \<omega>\<rangle> \<Longrightarrow>
             \<lparr> interp.domains = D, predicates = \<Delta>, funs = F \<rparr> \<Turnstile> \<langle>B; \<omega>\<rangle>"
-      and "\<And>D :: 'v domain_interp. \<And>F :: 'v fun_interp. \<And>\<omega> :: 'v state.
+      and "\<And>D :: 'v domain_interp. \<And>F :: 'v fun_interp. \<And>\<omega> :: 'v equi_state.
             fun_interp_indep_mask F \<Longrightarrow>
             \<lparr> interp.domains = D, predicates = \<Delta>, funs = F \<rparr> \<Turnstile> \<langle>B; \<omega>\<rangle> \<Longrightarrow>
             \<lparr> interp.domains = D, predicates = \<Delta>, funs = F \<rparr> \<Turnstile>[sem] \<langle>A^p; \<omega>\<rangle>"
@@ -988,17 +998,17 @@ next
     assume ?SEM
     then obtain \<omega>p where "I \<Turnstile> \<langle>ForAll x1a A; \<omega>p\<rangle>" "\<omega> = Abs_preal p \<odot> \<omega>p"
       using sat_sem_mult_def by blast
-    then have "\<And>v. v \<in> set_from_type (domains I) x1a \<Longrightarrow> I \<Turnstile> \<langle>syntactic_mult p A; shift_and_add_state \<omega> v\<rangle>"
+    then have "\<And>v. v \<in> set_from_type (domains I) x1a \<Longrightarrow> I \<Turnstile> \<langle>syntactic_mult p A; shift_and_add_equi_state \<omega> v\<rangle>"
     proof -
       fix v
       assume "v \<in> set_from_type (domains I) x1a"
-      then have "I \<Turnstile> \<langle>A; shift_and_add_state \<omega>p v\<rangle>"
+      then have "I \<Turnstile> \<langle>A; shift_and_add_equi_state \<omega>p v\<rangle>"
         using \<open>I \<Turnstile> \<langle>ForAll x1a A; \<omega>p\<rangle>\<close> by auto
-      moreover have "shift_and_add_state \<omega> v = Abs_preal p \<odot> (shift_and_add_state \<omega>p v)"
-        by (simp add: \<open>\<omega> = Abs_preal p \<odot> \<omega>p\<close> mult_shift_and_add_state_interchange)
-      ultimately have "I \<Turnstile>[sem] \<langle>A^Abs_preal p; shift_and_add_state \<omega> v\<rangle>"
+      moreover have "shift_and_add_equi_state \<omega> v = Abs_preal p \<odot> (shift_and_add_equi_state \<omega>p v)"
+        by (simp add: \<open>\<omega> = Abs_preal p \<odot> \<omega>p\<close> mult_shift_and_add_equi_state_interchange)
+      ultimately have "I \<Turnstile>[sem] \<langle>A^Abs_preal p; shift_and_add_equi_state \<omega> v\<rangle>"
         using sat_sem_mult_def by blast
-      then show "I \<Turnstile> \<langle>syntactic_mult p A; shift_and_add_state \<omega> v\<rangle>"
+      then show "I \<Turnstile> \<langle>syntactic_mult p A; shift_and_add_equi_state \<omega> v\<rangle>"
         by (simp add: ForAll)
     qed
     then show ?SYN
@@ -1010,17 +1020,17 @@ next
     let ?\<omega>p = "Abs_preal q \<odot> \<omega>"
     have "\<omega> = Abs_preal p \<odot> ?\<omega>p"
       by (metis \<open>q * p = 1\<close> assms(1) less_numeral_extra(1) mult.commute mult_inv_on_state_and_expr(1) zero_less_mult_pos2)
-    have "\<And>v. v \<in> set_from_type (domains I) x1a \<Longrightarrow> I \<Turnstile> \<langle>A; shift_and_add_state ?\<omega>p v\<rangle>"
+    have "\<And>v. v \<in> set_from_type (domains I) x1a \<Longrightarrow> I \<Turnstile> \<langle>A; shift_and_add_equi_state ?\<omega>p v\<rangle>"
     proof -
       fix v
       assume "v \<in> set_from_type (domains I) x1a"
-      then have "I \<Turnstile> \<langle>syntactic_mult p A; shift_and_add_state \<omega> v\<rangle>"
+      then have "I \<Turnstile> \<langle>syntactic_mult p A; shift_and_add_equi_state \<omega> v\<rangle>"
         using \<open>I \<Turnstile> \<langle>syntactic_mult p (ForAll x1a A); \<omega>\<rangle>\<close> by auto
-      then have "I \<Turnstile>[sem] \<langle>A^Abs_preal p; shift_and_add_state \<omega> v\<rangle>"
+      then have "I \<Turnstile>[sem] \<langle>A^Abs_preal p; shift_and_add_equi_state \<omega> v\<rangle>"
         by (simp add: ForAll)
-      moreover have "shift_and_add_state \<omega> v = Abs_preal p \<odot> (shift_and_add_state ?\<omega>p v)"
-        by (metis \<open>\<omega> = Abs_preal p \<odot> ?\<omega>p\<close> mult_shift_and_add_state_interchange)
-      ultimately show " I \<Turnstile> \<langle>A; shift_and_add_state ?\<omega>p v\<rangle>"
+      moreover have "shift_and_add_equi_state \<omega> v = Abs_preal p \<odot> (shift_and_add_equi_state ?\<omega>p v)"
+        by (metis \<open>\<omega> = Abs_preal p \<odot> ?\<omega>p\<close> mult_shift_and_add_equi_state_interchange)
+      ultimately show " I \<Turnstile> \<langle>A; shift_and_add_equi_state ?\<omega>p v\<rangle>"
         using assms(1) sat_sem_mult_def mult_inv_on_state_implies_uniqueness by blast
     qed
     then show ?SEM
@@ -1033,13 +1043,13 @@ next
     assume ?SEM
     then obtain \<omega>p where "I \<Turnstile> \<langle>Exists x1a A; \<omega>p\<rangle>" "\<omega> = Abs_preal p \<odot> \<omega>p"
       using sat_sem_mult_def by blast
-    then obtain v where "v \<in> set_from_type (domains I) x1a" "I \<Turnstile> \<langle>A; shift_and_add_state \<omega>p v\<rangle>"
+    then obtain v where "v \<in> set_from_type (domains I) x1a" "I \<Turnstile> \<langle>A; shift_and_add_equi_state \<omega>p v\<rangle>"
       using sat.simps(7) by blast
-    moreover have "shift_and_add_state \<omega> v = Abs_preal p \<odot> (shift_and_add_state \<omega>p v)"
-      by (simp add: \<open>\<omega> = Abs_preal p \<odot> \<omega>p\<close> mult_shift_and_add_state_interchange)
-    ultimately have "I \<Turnstile>[sem] \<langle>A^Abs_preal p; shift_and_add_state \<omega> v\<rangle>"
+    moreover have "shift_and_add_equi_state \<omega> v = Abs_preal p \<odot> (shift_and_add_equi_state \<omega>p v)"
+      by (simp add: \<open>\<omega> = Abs_preal p \<odot> \<omega>p\<close> mult_shift_and_add_equi_state_interchange)
+    ultimately have "I \<Turnstile>[sem] \<langle>A^Abs_preal p; shift_and_add_equi_state \<omega> v\<rangle>"
       using sat_sem_mult_def by blast
-    then have "I \<Turnstile> \<langle>syntactic_mult p A; shift_and_add_state \<omega> v\<rangle>"
+    then have "I \<Turnstile> \<langle>syntactic_mult p A; shift_and_add_equi_state \<omega> v\<rangle>"
       by (simp add: Exists)
     then show ?SYN
       using \<open>v \<in> set_from_type (interp.domains I) x1a\<close> by auto
@@ -1050,14 +1060,14 @@ next
     let ?\<omega>p = "Abs_preal q \<odot> \<omega>"
     have "\<omega> = Abs_preal p \<odot> ?\<omega>p"
       by (metis \<open>q * p = 1\<close> assms(1) less_numeral_extra(1) mult.commute mult_inv_on_state_and_expr(1) zero_less_mult_pos2)
-    moreover obtain v where "v \<in> set_from_type (domains I) x1a" "I \<Turnstile> \<langle>syntactic_mult p A; shift_and_add_state \<omega> v\<rangle>"
+    moreover obtain v where "v \<in> set_from_type (domains I) x1a" "I \<Turnstile> \<langle>syntactic_mult p A; shift_and_add_equi_state \<omega> v\<rangle>"
       using \<open>I \<Turnstile> \<langle>syntactic_mult p (Exists x1a A); \<omega>\<rangle>\<close> by auto
-    ultimately have "I \<Turnstile> \<langle>A; shift_and_add_state ?\<omega>p v\<rangle>"
+    ultimately have "I \<Turnstile> \<langle>A; shift_and_add_equi_state ?\<omega>p v\<rangle>"
     proof -
-      have "I \<Turnstile>[sem] \<langle>A^Abs_preal p; shift_and_add_state \<omega> v\<rangle>"
-        by (simp add: Exists \<open>I \<Turnstile> \<langle>syntactic_mult p A; shift_and_add_state \<omega> v\<rangle>\<close>)
-      moreover have "shift_and_add_state \<omega> v = Abs_preal p \<odot> (shift_and_add_state ?\<omega>p v)"
-        by (metis \<open>\<omega> = Abs_preal p \<odot> ?\<omega>p\<close> mult_shift_and_add_state_interchange)
+      have "I \<Turnstile>[sem] \<langle>A^Abs_preal p; shift_and_add_equi_state \<omega> v\<rangle>"
+        by (simp add: Exists \<open>I \<Turnstile> \<langle>syntactic_mult p A; shift_and_add_equi_state \<omega> v\<rangle>\<close>)
+      moreover have "shift_and_add_equi_state \<omega> v = Abs_preal p \<odot> (shift_and_add_equi_state ?\<omega>p v)"
+        by (metis \<open>\<omega> = Abs_preal p \<odot> ?\<omega>p\<close> mult_shift_and_add_equi_state_interchange)
       ultimately show ?thesis
         using assms(1) sat_sem_mult_def mult_inv_on_state_implies_uniqueness by blast
     qed
